\documentclass{scrartcl}

\input{./packages}
\input{./definitions}
\newcommand{\exercise}[2]{\vspace{1em}\noindent{\bf Exercise #1 (#2)}}
\renewcommand{\proof}{\vspace{0.8em}\noindent{\bf Proof: }}

\begin{document}
\noindent{\footnotesize Computer Graphics 2014/15, Exercise 10} 
\hfill 
{\footnotesize \input{./currentDate.txt}}
\newline
{\footnotesize \input{../../NAMES.txt}}

\noindent\hrulefill

\exercise{10.3}{Bernstein basis to Monom basis }\\
$\begin{pmatrix}
B_0^n(t)\\
\vdots\\
B_n^n(t)
\end{pmatrix} =C\begin{pmatrix}
1\\t\\t\\t^2\\\vdots\\t^n
\end{pmatrix}$ with $C_{i,j}=\binom{j}{i}\binom{n}{j}(-1)^{j-i}$
\begin{equation}
(a+b)^n=\sum_{k=0}^{n}\binom{n}{k}a^{n-k}b^k \label{binom}
\end{equation}
\begin{align*}
	B_i^n(t)&=\sum_{j=0}^{n}C_{i,j}t^j\\&=\sum_{j=0}^{n}\binom{j}{i}\binom{n}{j}(-1)^{j-i}t^j\stackrel{\binom{j}{i}=0\text{ for }  i>j}{=} \sum_{j=i}^{n}\frac{n!j!}{(n-j)!j!(j-i)!}(-1)^{j-i}t^{j-i}t^i\\
	&=t^i\frac{n!}{i!(n-i)!}\sum_{j=i}^{n}\frac{(n-i)!}{(n-j)!(j-i)!}(-t)^{j-i}(1)^{n-j}\\
	& \stackrel{j\rightarrow j+i}{=}t^i\binom{n}{i}\sum_{j=0}^{n-i}\frac{(n-i)!}{(n-i-j)!j!}(-t)^{j}(1)^{n-i-j}\\
	&\stackrel{\ref{binom}}{=} \binom{n}{i}t^i(1-t)^{n-i}
\end{align*}
	

\end{document}
