\documentclass{scrartcl}

\input{./packages}
\input{./definitions}
\newcommand{\exercise}[2]{\vspace{1em}\noindent{\bf Exercise #1 (#2)}}
\renewcommand{\proof}{\vspace{0.8em}\noindent{\bf Proof: }}

\begin{document}
\noindent{\footnotesize Computer Graphics 2014/15, Exercise 9} 
\hfill 
{\footnotesize \input{./currentDate.txt}}
\newline
{\footnotesize \input{../../NAMES.txt}}

\noindent\hrulefill

\exercise{9.4}{Tangent}
	\\\begin{align*}
		x(t)=&\sum_{i=0}^{n}B_i^n(t)P_i\\	%\hspace{10mm}
		\partial_t:=&\frac{\partial}{\partial_t}\\
		\binom{n}{i}=&\frac{n!}{i!(n-i)!}\\	
		\partial_t x(t)=&\sum_{i01}^{n}\partial_t B_i^n(t)P_i\\
		=&\sum_{i=0}^{n}\partial_t \left(  \binom{n}{i} t^i (1-t)^{n-i} \right) P_i\\
		=&\sum_{i=1}^{n} \left(  \binom{n}{i}i t^{i-1} (1-t)^{n-i} \right) P_i-\sum_{i=0}^{n} \left(  \binom{n}{i} t^i(n-i) (1-t)^{n-i-1} \right) P_i\\
		=& n\left( \sum_{i=1}^{n}\frac{(n-1)!}{(i-1)!(n-i)!}t^{i-1}(1-t)^{n-i}P_i-\sum_{i=0}^{n-1}\frac{(n-1)!}{i!(n-i-1)!}t^i(1-t)^{n-i-1}P_i\right)\\
		=& n\left(\sum_{i=0}^{n-1}\frac{(n-1)!}{i!(n-(i+1))!}t^{i}(1-t)^{n-(i+1)}P_{i+1}-\sum_{i=0}^{n-1}\binom{n-1}{i}t^i(1-t)^{(n-1)-i}P_i\right)\\ 
		=& n\left(\sum_{i=0}^{n-1}\binom{n-1}{i}t^{i}(1-t)^{(n-1)-i}P_{i+1}-\sum_{i=0}^{n-1}\binom{n-1}{i}t^i(1-t)^{(n-1)-i}P_i\right)\\ 
		=& n\sum_{i=0}^{n-1}B^{n-1}_i(t)(P_{i+1}-P_i)\\
		n'=& n-1\\
		\stackrel{-}{P}_i=& (P_{i+1}-P_i)n\\
		\stackrel{.}{x}(t)=&\sum_{i=0}^{n'}B^{n'}_i\stackrel{-}{P}_i\\
		\stackrel{.}{x}(0)=&\stackrel{-}{P}_0=n(P_1-P_0)\\
		\stackrel{.}{x}(1)=&\stackrel{-}{P}_{n'}=n(P_n-P_{n-1})			
	\end{align*}
	Tangent in $x(0)$: $g(s)~=P_0+\stackrel{.}{x}(0)*l$\\
	Tangent in $x(1)$: $g'(s)=P_n+\stackrel{.}{x}(1)*l$\\
	$P_1=g(\tfrac{1}{n})$ $\Rightarrow$ Tangent in $x(0)$ points in direction of $P_1-P_0$\\
	$P_{n-1}=g'(-\tfrac{1}{n})$ $\Rightarrow$ Tangent in $x(1)$ points in direction of $P_{n-1}-P_n$


\end{document}
